src/trace.v
@@ -1,0 +1,119 @@
+From ITree Require Import ITree Eqit.
+From stdpp Require Import list.
+From iris.itree Require Import axioms itree.
+From Paco Require Import paco.
+From Paco Require Import paco2.
+From Coq Require Import ssreflect.
+
+Inductive trace (E : Type → Type) (R : Type) :=
+  | TRet (r : R)
+  | TVis (A : Type) (e : E A) (a : A) (k : trace E R)
+  | TVisEmpty (A : Type) (e : E A)
+  | TCut.
+
+Arguments TRet {_ _}.
+Arguments TVis {_ _}.
+Arguments TVisEmpty {_ _}.
+Arguments TCut {_ _}.
+
+Section is_trace.
+  Context {E : Type → Type} {R : Type}.
+
+  Inductive is_trace_
+    : trace E R
+    → itree' E R
+    → Prop :=
+  | is_TRet r :
+    is_trace_ (TRet r) (RetF r)
+  | is_TVis tr' A (e : E A) a k :
+    is_trace_ tr' (observe (k a)) →
+    is_trace_ (TVis A e a tr') (VisF e k)
+  | is_TVisEmpty A (f : A → Empty_set) (e : E A) k :
+    is_trace_ (TVisEmpty A e) (VisF e k)
+  | is_TCut t :
+    is_trace_ TCut t
+  | trace_skip_tau tr t' :
+    is_trace_ tr (observe t') →
+    is_trace_ tr (TauF t').
+
+  Definition is_trace (tr : trace E R) (t : itree E R) : Prop :=
+    is_trace_ tr (observe t).
+
+  Local Instance is_trace_eutt_unilateral :
+    Proper (pointwise_relation (trace E R) (eutt (=) ==> impl)) is_trace.
+  Proof.
+    intros tr t1 t2 Heqit Htr.
+    rewrite /is_trace. rewrite /is_trace in Htr.
+    remember (observe t1) as ot1. remember (observe t2) as ot2.
+    revert t1 t2 ot2 Heqot1 Heqot2 Heqit. induction Htr as [r|tr' A e a k Htr IH|A f e k|t|tr t' Htr IH]; intros t1 t2 ot2 Heqot1 Heqot2 Heqit.
+    - punfold Heqit. rewrite /eqit_ in Heqit. remember (observe t1) as ot1. destruct Heqot2.
+      induction Heqit as [r1 r2| | | | ot1 t2' _ _ IH ]; try discriminate.
+      * injection Heqot1 as ->. destruct REL. constructor.
+      * constructor. by apply IH.
+    - punfold Heqit. rewrite /eqit_ in Heqit. remember (observe t1) as ot1. destruct Heqot2.
+      induction Heqit as [ | | B e' k1 k2 REL | | ot1 t2' _ _ IH' ]; try discriminate.
+      * simplify_K. simplify_K. constructor. apply IH with (t1 := k1 a) (t2 := k2 a); try done.
+        pclearbot. apply REL.
+      * constructor. by apply IH'.
+    - punfold Heqit. rewrite /eqit_ in Heqit. remember (observe t1) as ot1. destruct Heqot2.
+      induction Heqit as [ | | B e' k1 k2 REL | | ot1 t2' _ _ IH' ]; try discriminate.
+      * simplify_K. simplify_K. by constructor.
+      * constructor. by apply IH'.
+    - punfold Heqit. rewrite /eqit_ in Heqit. remember (observe t1) as ot1. destruct Heqot2.
+      induction Heqit as [ | | B e' k1 k2 REL | | ot1 t2' _ _ IH' ]; try discriminate; constructor.
+    - apply IH with (t1 := t') (t2 := t2); eauto.
+      transitivity (Tau t'). { apply eqit_inv_Tau_l. reflexivity. }
+      pfold. rewrite /eqit_. simpl. rewrite Heqot1. punfold Heqit.
+  Qed.
+  Global Instance is_trace_eutt :
+    Proper (pointwise_relation (trace E R) (eutt (=) ==> (↔))) is_trace.
+  Proof.
+    intros tr t1 t2 Heqit. split; apply is_trace_eutt_unilateral.
+    - done.
+    - by symmetry.
+  Qed.
+End is_trace.
+
+Class AnswerEqDecision (E : Type → Type) :=
+  is_AnswerEqDecision A : E A → EqDecision A.
+
+Global Instance AnswerEqDecisionSum E E' :
+  AnswerEqDecision E →
+  AnswerEqDecision E' →
+  AnswerEqDecision (E +' E').
+Admitted.
+
+Program Definition equal `{AnswerEqDecision E} {A : Type} (e : E A) (a a' : A) : {a = a'} + {a ≠ a'} :=
+  @decide (a = a') _.
+Next Obligation.
+  intros E Hdec A e a a'. by apply is_AnswerEqDecision.
+Qed.
+
+Fixpoint interp_tr {R E E'} (tr : trace (E +' E') R) : trace E' R :=
+  match tr with
+  | TRet r => TRet r
+  | TVis A (inl1 e) _ k => interp_tr k
+  | TVis A (inr1 e) a k => TVis A e a (interp_tr k)
+  | TVisEmpty A (inl1 e) =>  (* Placeholder: *) TCut
+  | TVisEmpty A (inr1 e) => TVisEmpty A e
+  | TCut => TCut
+  end.
+
+Inductive is_postfix {E R}
+  : trace E R
+  → trace E R
+  → Prop :=
+| is_postfix_same tr :
+  is_postfix tr tr
+| is_postfix_TVis tr tr' A e a :
+  is_postfix tr tr' →
+  is_postfix tr (TVis A e a tr').
+
+Global Instance is_postfix_trans {E R} :
+  Transitive (is_postfix (E:=E) (R:=R)).
+Admitted.
+
+Lemma interp_tr_is_postfix {E E' R} (tr tr' : trace (E +' E') R) :
+  is_postfix tr tr' →
+  is_postfix (interp_tr tr) (interp_tr tr').
+Admitted.
